Format code and restate goals

Doubly_Linked_List_VST.v
@@ -5,736 +5,725 @@
 
     struct node;
     struct list;
-    struct node * begin(struct list * );
-    struct node * end(struct list * );
-    struct node * next(struct node * );
-    struct node * rbegin(struct list * );
-    struct node * rend(struct list * );
-    struct node * rnext(struct node * );
-    unsigned int get_val(struct node * );
-    void insert_before (struct list *, struct node *; unsigned int )
-    void insert_after (struct list *, struct node *; unsigned int )
+    struct list *list_new();
+    void list_free(struct list *l);
+    struct node *begin(struct list *l);
+    struct node *end(struct list *l);
+    struct node *rbegin(struct list *l);
+    struct node *rend(struct list *l);
+    struct node *next(struct node *p);
+    struct node *rnext(struct node *p);
+    unsigned int get_val(struct node *p);
+    
+    void insert_before(struct list *l, struct node *p, unsigned int v);
+    void insert_after(struct list *l, struct node *p, unsigned int v);
+    void merge(struct list *l1, struct list *l2);
 
     You may change the definition below if your version is better. *)
-    Require Import EV.dlinklist.
-    Require Import VST.floyd.proofauto.
-    
-    Instance CompSpecs : compspecs. make_compspecs prog. Defined.
-    Definition Vprog : varspecs. mk_varspecs prog. Defined.
-    
-    Definition t_struct_node : type := Tstruct _node noattr.
-    Definition t_struct_list : type := Tstruct _list noattr.
-    
-    (** Concrete memory representation of a dlinklist, which does not only include
-        value but also include addresses. *)
-    
-    Fixpoint dlrep (l : list (Z * val)) (head tail prev next : val) : mpred :=
-      match l with
-      | (x, p) :: l' =>
-          EX head' : val,
-            !! (p = head) &&
-            data_at Tsh t_struct_node (Vint (Int.repr x), (prev, head')) head *
-            dlrep l' head' tail head next
-      | nil => !! (tail = prev /\ head = next) && emp
-      end.
-      
-    
-    
-    (** Memory representation of a mathematical list. Cursors mean places to
-        insert. *)
-    Definition list_rep_with_cursor (l : list (Z * val)) (p : val) : mpred :=
-      EX (head tail : val),
-        data_at Tsh t_struct_list (head, tail) p *
-          dlrep l head tail nullval nullval.
-    
-    Definition list_rep (l : list Z) (p : val) : mpred :=
-      EX l0: list (Z * val),
-        !! (map fst l0 = l) && list_rep_with_cursor l0 p.
-        
-        
-    Fixpoint dlseg (sigma: list (Z * val)) (head tail: val) : mpred :=
-      match sigma with
-      | nil => !! (head = tail) && emp
-      | (x,p)::hs => EX prev next:val, !!(p=head) && data_at Tsh t_struct_node (Vint (Int.repr x), (prev, next)) head * dlseg hs next tail
-      end.
-      
-    (*
-      dlrep_singleton: for a dlist with only one element (x, y), it's equivalent to 
-                       data_at y. 
-    *)
-    Lemma dlrep_singleton: forall x y head tail prev next,
-      
-        dlrep [(x,y)] head tail prev next |-- !! (head = tail /\ head = y) && data_at Tsh t_struct_node (Vint (Int.repr x), (prev, next)) y .
-    Proof.
-      intros.
-      unfold dlrep.
-      Intros head'.
-      entailer!.
-    Qed.
-    
-    Lemma singleton_dlrep (x : Z) ( y head tail prev next : val):
-      !! (head = tail /\ head = y) && data_at Tsh t_struct_node (Vint (Int.repr x), (prev, next)) y |-- dlrep [(x,y)] head tail prev next.
-    Proof.
-      intros.
-      unfold dlrep.
-      Exists next.
-      entailer!.
-    Qed.
-    
-    
-    (* 
-           Lemma dlrep_left_elem.
-    
-           dlinklist layout: 
-                | data_at | |------------dlrep l next  tail p nx------------|
-           pv <-> (v, p) <-> (v1, p1) <-> (v2, p2) <-> ...... <-> (v_n, p_n) <-> nx
-                   head        next                                   tail 
-                  |-------------dlrep (v,p)::l head tail pv nx -------------|   
-     *)
-    Lemma dlrep_left_elem (l2: list (Z * val)) (v:Z) (p head tail pv nx: val): 
-      dlrep ((v,p) :: l2) head tail pv nx |-- 
-      EX next,
-        !!(p = head) && emp * 
-        dlrep l2 next tail p nx *
-        data_at Tsh t_struct_node (Vint (Int.repr v), (pv, next)) p.
-          
-    Proof.
-      intros.
-      destruct l2.
-      sep_apply (dlrep_singleton).
-      unfold dlrep; fold dlrep.
-      Exists nx.
-      entailer!.
-      
-      unfold dlrep. fold dlrep.
-      Intros head'.
-      Exists head'.
-      entailer!.
-    Qed.
-    
-    (* Similar with dlrep_left_elem,
-           but the parameters on the left and right side of `|--` are switched *)
-    Lemma elem_left_dlrep (l2: list (Z * val)) (v:Z) (p head tail pv nx next: val):
-      !! (p = head) && emp * 
-        dlrep l2 next tail p nx *
-        data_at Tsh t_struct_node (Vint (Int.repr v), (pv, next)) p |-- dlrep ((v,p) :: l2) head tail pv nx.
-    Proof.
-      intros.
-      entailer!.
-      destruct l2.
-      unfold dlrep.
-      Exists next.
-      entailer!.
-      
-      unfold dlrep; fold dlrep.
-      destruct p.
-      Intros head'.
-      Exists next.
-      Exists head'.
-      entailer!.
-    Qed.
-      
-    
-    Require Import Coq.Classes.RelationClasses.
-    Require Import Coq.Classes.Morphisms.
-    Require Import PL.Imp.
-       
-    Check data_at.
-    
-    (** Head pointer and tail pointer *)
-    Definition head_with_default {A: Type} (l: list A) (default: A): A :=
-      match l with
-      | a :: _ => a
-      | nil => default
-      end.
-    
-    Definition head_ptr (l : list (Z * val)): val :=
-      head_with_default (map snd l) nullval.
-      
-    Definition tail_ptr (l : list (Z * val)): val :=
-      head_with_default (rev (map snd l)) nullval.
-      
-    Lemma elem_right_dlrep (l2 : list (Z * val)) (v : Z) (p head tail pv nx prev: val):
+
+Require Import VST.floyd.proofauto.
+Require Import EV.dlinklist.
+
+Instance CompSpecs : compspecs. make_compspecs prog. Defined.
+Definition Vprog : varspecs. mk_varspecs prog. Defined.
+
+Definition t_struct_node : type := Tstruct _node noattr.
+Definition t_struct_list : type := Tstruct _list noattr.
+
+(** Concrete memory representation of a dlinklist, which does not only include
+    value but also include addresses. *)
+
+Fixpoint dlrep (l : list (Z * val)) (head tail prev next : val) : mpred :=
+  match l with
+  | (x, p) :: l' =>
+      EX head' : val,
+        !! (p = head) &&
+        data_at Tsh t_struct_node (Vint (Int.repr x), (prev, head')) head *
+        dlrep l' head' tail head next
+  | nil => !! (tail = prev /\ head = next) && emp
+  end.
+
+(* Some basic properties about dlrep. *)
+
+Lemma dlrep_singleton:
+  forall x y head tail prev next,
+    dlrep [(x, y)] head tail prev next |--
+    !! (head = tail /\ head = y) &&
+    data_at Tsh t_struct_node (Vint (Int.repr x), (prev, next)) y.
+Proof.
+  intros.
+  unfold dlrep.
+  Intros head'.
+  entailer!.
+Qed.
+
+Lemma singleton_dlrep:
+  forall x y head tail prev next,
+    !! (head = tail /\ head = y) &&
+    data_at Tsh t_struct_node (Vint (Int.repr x), (prev, next)) y |--
+    dlrep [(x, y)] head tail prev next.
+Proof.
+  intros.
+  unfold dlrep.
+  Exists next.
+  entailer!.
+Qed.
+
+Lemma dlrep_left_elem:
+  forall l x p head tail prev next,
+    dlrep ((x, p) :: l) head tail prev next |-- 
+    EX next',
+      !!(p = head) && emp * 
+      dlrep l next' tail p next *
+      data_at Tsh t_struct_node (Vint (Int.repr x), (prev, next')) p.
+Proof.
+  intros.
+  destruct l.
+  + sep_apply dlrep_singleton.
+    unfold dlrep; fold dlrep.
+    Exists next.
+    entailer!.
+  + unfold dlrep; fold dlrep.
+    Intros head'.
+    Exists head'.
+    entailer!.
+Qed.
+
+Lemma elem_left_dlrep:
+  forall l x p head tail prev next next',
+    !! (p = head) && emp * 
+    dlrep l next' tail p next *
+    data_at Tsh t_struct_node (Vint (Int.repr x), (prev, next')) p |--
+    dlrep ((x, p) :: l) head tail prev next.
+Proof.
+  intros.
+  entailer!.
+  destruct l.
+  + unfold dlrep; fold dlrep.
+    Exists next.
+    entailer!.
+  + unfold dlrep; fold dlrep.
+    destruct p.
+    Intros head'.
+    Exists next'.
+    Exists head'.
+    entailer!.
+Qed.
+
+Lemma dlrep_right_elem:
+  forall l x p head tail (prev: val) next,
+    dlrep (l ++ [(x, p)]) head tail prev next |-- 
+    EX p',
       !!(p = tail) && emp * 
-        dlrep l2 head prev pv p *
-        data_at Tsh t_struct_node (Vint (Int.repr v), (prev, nx)) p
-      |-- dlrep ( l2 ++ [(v,p)]) head tail pv nx.
-    Proof.
-      revert head tail pv nx prev.
-      induction l2; intros.
-      + simpl.
-        Exists nx.
+      dlrep l head p' prev p *
+      data_at Tsh t_struct_node (Vint (Int.repr x), (p', next)) p.
+Proof.
+  intros.
+  revert head tail prev next.
+  induction l; intros.
+  + autorewrite with sublist.
+    sep_apply dlrep_singleton.
+    Exists prev.
+    unfold dlrep; fold dlrep.
+    entailer!.
+  + unfold dlrep; fold dlrep.
+    destruct a.
+    simpl.
+    Intros head'.
+    specialize (IHl head' tail head next).
+    sep_apply IHl.
+    Intros p'.
+    Exists p' head'.
+    entailer!.
+Qed.
+
+Lemma elem_right_dlrep:
+  forall l x p head tail prev next prev',
+    !! (p = tail) && emp * 
+      dlrep l head prev' prev p *
+      data_at Tsh t_struct_node (Vint (Int.repr x), (prev', next)) p
+    |-- dlrep (l ++ [(x, p)]) head tail prev next.
+Proof.
+  intros.
+  revert head tail prev next prev'.
+  induction l; intros.
+  + simpl.
+    Exists next.
+    entailer!.
+  + unfold dlrep; fold dlrep.
+    destruct a.
+    Intros head'.
+    specialize (IHl head' tail head next prev').
+
+    assert_PROP (dlrep l head' prev' head p *
+      data_at Tsh t_struct_node (Vint (Int.repr x), (prev', next)) p |--
+      !! (p = tail) && emp * dlrep l head' prev' head p *
+      data_at Tsh t_struct_node (Vint (Int.repr x), (prev', next)) p).
+    { entailer!. }
+
+    sep_apply H1.
+    sep_apply IHl.
+    { exact H. }
+
+    simpl.
+    Exists head'.
+    entailer!.
+Qed.
+
+Lemma dlrep_middle_elem:
+  forall l1 x p l2 head tail prev next, 
+    dlrep (l1 ++ (x, p) :: l2) head tail prev next |-- EX prev' next',
+      dlrep l1 head prev' prev p * 
+      data_at Tsh t_struct_node (Vint (Int.repr x), (prev', next')) p *
+      dlrep l2 next' tail p next.
+Proof.
+  intros.
+  revert head tail prev next.
+  induction l1, l2; intros; autorewrite with sublist; unfold dlrep; fold dlrep.
+  + Intros next'.
+    Exists prev next.
+    entailer!.
+  + Intros next'.
+    Exists prev next'.
+    entailer!.
+  + assert ((a :: l1) ++ [(x, p)] = a :: (l1 ++ [(x, p)])).
+    list_solve.
+    rewrite H.
+    pose proof dlrep_left_elem.
+    destruct a.
+    specialize (H0 (l1 ++ [(x, p)]) z v head tail prev next).
+    sep_apply H0.
+    Intros next'.
+    specialize (IHl1 next' tail v next).
+    sep_apply IHl1.
+    Intros prev' next'0.
+    Exists prev' next'0.
+    Exists next'.
+    unfold dlrep; fold dlrep.
+    entailer!.
+  + pose proof dlrep_left_elem.
+    destruct a.
+    assert (((z, v) :: l1) ++ (x, p) :: p0 :: l2 = (z, v) :: l1 ++ (x, p) :: p0 :: l2).
+    list_solve.
+    rewrite H0; clear H0.
+    specialize (H (l1 ++ (x, p) :: p0 :: l2) z v head tail prev next).
+    sep_apply H.
+    Intros next'.
+    specialize (IHl1 next' tail v next).
+    sep_apply IHl1.
+    Intros prev' next'0.
+    Exists prev' next'0.
+    Exists next'.
+    destruct p0.
+    pose proof dlrep_left_elem.
+    specialize (H1 l2 z0 v0 next'0 tail p next).
+    sep_apply H1.
+    Intros next'1.
+    Exists next'1.
+    entailer!.
+Qed.
+
+Lemma elem_middle_dlrep:
+  forall l1 l2 x p head tail prev next prev' next',
+    dlrep l1 head prev' prev p * 
+      data_at Tsh t_struct_node (Vint (Int.repr x), (prev', next')) p *
+      dlrep l2 next' tail p next
+    |-- dlrep (l1 ++ (x, p) :: l2) head tail prev next.
+Proof.
+  intros.
+  revert head tail prev next prev' next' p x.
+  induction l1, l2; intros; autorewrite with sublist; unfold dlrep; fold dlrep.
+  + Exists next'.
+    entailer!.
+  + destruct p.
+    Intros head'.
+    Exists next' head'.
+    entailer!.
+  + assert ((a :: l1) ++ [(x, p)] = a :: (l1 ++ [(x, p)])).
+    list_solve.
+    rewrite H.
+    destruct a.
+    pose proof elem_left_dlrep.
+    specialize (H0 (l1 ++ [(x, p)]) z v head tail prev next).
+    Intros head'.
+    specialize (H0 head').
+    assert_PROP (data_at Tsh t_struct_node (Vint (Int.repr z), (prev, head')) head *
+      dlrep l1 head' prev' head p *
+      data_at Tsh t_struct_node (Vint (Int.repr x), (prev', next')) p * emp |--
+      !! (v = head) && emp * dlrep (l1 ++ [(x, p)]) head' tail v next *
+      data_at Tsh t_struct_node (Vint (Int.repr z), (prev, head')) v).
+    - entailer!.
+      cancel.
+      specialize (IHl1 head' p head next prev' next p x).
+      assert_PROP (dlrep l1 head' prev' head p *
+        data_at Tsh t_struct_node (Vint (Int.repr x), (prev', next)) p |--
+        dlrep l1 head' prev' head p *
+        data_at Tsh t_struct_node (Vint (Int.repr x), (prev', next)) p *
+        dlrep [] next p p next).
+      * unfold dlrep; fold dlrep.
         entailer!.
-      + unfold dlrep; fold dlrep.
-        autorewrite with norm.
-        destruct a.
-        Intros head'.
-        specialize (IHl2 head' tail head nx prev).
-        assert_PROP ( dlrep l2 head' prev head p *
-    data_at Tsh t_struct_node (Vint (Int.repr v), (prev, nx)) p |-- !! (p = tail) && emp * dlrep l2 head' prev head p *
-           data_at Tsh t_struct_node (Vint (Int.repr v), (prev, nx)) p).
+        entailer!. 
+      * sep_apply H1.
+        sep_apply IHl1.
         entailer!.
-        sep_apply H1.
-        sep_apply IHl2.
-        exact H.
-        simpl.
-        Exists head'.
-        entailer!.
-    Qed.
-    
-    (* Similar with dlrep_left_elem, but (v,p) is at the right size of the dlinklist *)
-    Lemma dlrep_right_elem: forall l2 v p head tail pv nx, 
-      dlrep ( l2 ++ [(v,p)]) head tail pv nx |-- 
-      EX prev,
-        !!(p = tail) && emp * 
-        dlrep l2 head prev pv p *
-        
-        data_at Tsh t_struct_node (Vint (Int.repr v), (prev, nx)) p.
-          
-    Proof.
-      intros.
-      revert head tail pv nx.
-      induction l2; intros.
-      autorewrite with sublist.
-      sep_apply (dlrep_singleton).
-      Exists pv.
-      unfold dlrep; fold dlrep.
+    - sep_apply H4.
+      sep_apply H0.
+      exact H3.
       entailer!.
-      
-      unfold dlrep. fold dlrep.
-      autorewrite with norm.
-      destruct a.
-      simpl.
-      Intros  headof_l2.
-      
-      specialize (IHl2 headof_l2 tail head nx).
-      sep_apply IHl2.
-      simpl.
-      Intros prev.
-      Exists prev headof_l2.
-      entailer!.   
-    Qed.
-    
-    (* Similar with elem_left_dlrep, but (p,v) is in the middle of two dlinklist *)
-    Lemma elem_middle_dlrep (l1 l2 : list (Z * val)) (v : Z) (p head tail pv nx prev next: val):
-      dlrep l1 head prev pv p * 
-            data_at Tsh t_struct_node (Vint (Int.repr v), (prev, next)) p *
-            dlrep l2 next tail p nx |-- dlrep (l1 ++ (v,p) :: l2) head tail pv nx.
-    Proof.
-      revert head tail pv nx prev next p v.
-      induction l1, l2; intros; autorewrite with sublist; unfold dlrep; fold dlrep.
-      + Exists next.
-      entailer!.
-      + destruct p.
-        Intros head'.
-        Exists next head'.
+  + destruct a, p.
+    assert (((z, v) :: l1) ++ (x, p0) :: (z0, v0) :: l2 = (z, v) :: l1 ++ (x, p0) :: (z0, v0) :: l2).
+    list_solve.
+    rewrite H; clear H.
+    pose proof elem_left_dlrep.
+    Intros l1_head l2_head.
+    specialize (H (l1 ++ (x, p0) :: (z0, v0) :: l2) z v head tail prev next l1_head).
+    assert_PROP (data_at Tsh t_struct_node (Vint (Int.repr z), (prev, l1_head)) head *
+      dlrep l1 l1_head prev' head p0 *
+      data_at Tsh t_struct_node (Vint (Int.repr x), (prev', next')) p0 *
+      (data_at Tsh t_struct_node (Vint (Int.repr z0), (p0, l2_head)) next' *
+        dlrep l2 l2_head tail next' next) |--
+      !! (v = head) && emp *
+      dlrep (l1 ++ (x, p0) :: (z0, v0) :: l2) l1_head tail v next *
+      data_at Tsh t_struct_node (Vint (Int.repr z), (prev, l1_head)) v).
+    - entailer!.
+      pose proof elem_left_dlrep.
+      specialize (H0 l2 z0 next' next' tail p0 next l2_head).
+      assert_PROP (data_at Tsh t_struct_node (Vint (Int.repr z0), (p0, l2_head)) next' *
+        dlrep l2 l2_head tail next' next |--
+        !! (next' = next') && emp * dlrep l2 l2_head tail next' next *
+        data_at Tsh t_struct_node (Vint (Int.repr z0), (p0, l2_head)) next').
+      * entailer!.
         entailer!.
-      + assert ((a :: l1) ++ [(v,p)] = a :: (l1 ++ [(v,p)])).
-        list_solve.
-        rewrite H.
-        destruct a.
-        pose proof elem_left_dlrep.
-        specialize (H0 (l1++[(v,p)]) z v0 head tail pv nx).
-        Intros head'.
-        specialize (H0 head').
-        assert_PROP ( data_at Tsh t_struct_node (Vint (Int.repr z), (pv, head')) head *
-    dlrep l1 head' prev head p *
-    data_at Tsh t_struct_node (Vint (Int.repr v), (prev, next)) p * emp|--!! (v0 = head) && emp * dlrep (l1 ++ [(v, p)]) head' tail v0 nx *
-         data_at Tsh t_struct_node (Vint (Int.repr z), (pv, head')) v0).
-         entailer!.
-         cancel.
-         specialize (IHl1 head' p head nx prev nx p v).
-         assert_PROP(dlrep l1 head' prev head p *
-    data_at Tsh t_struct_node (Vint (Int.repr v), (prev, nx)) p|--dlrep l1 head' prev head p *
-           data_at Tsh t_struct_node (Vint (Int.repr v), (prev, nx)) p *
-           dlrep [] nx p p nx).
-         unfold dlrep; fold dlrep. entailer!. entailer!. 
-         sep_apply H1. sep_apply IHl1. entailer!.
-         sep_apply H4.
-         sep_apply H0.
-         exact H3.
-         entailer!.
-       + destruct a, p.
-         assert (((z, v0) :: l1) ++ (v, p0) :: (z0,v1) :: l2 = (z, v0) :: l1 ++ (v, p0) :: (z0,v1) :: l2).
-        list_solve.
-        rewrite H; clear H.
-        pose proof elem_left_dlrep.
-        Intros l1_head l2_head.
-        specialize (H (l1 ++ (v, p0) :: (z0, v1) :: l2) z v0 head tail pv nx l1_head).
-        
-        assert_PROP (data_at Tsh t_struct_node (Vint (Int.repr z), (pv, l1_head)) head *
-    dlrep l1 l1_head prev head p0 *
-    data_at Tsh t_struct_node (Vint (Int.repr v), (prev, next)) p0 *
-    (data_at Tsh t_struct_node (Vint (Int.repr z0), (p0, l2_head)) next *
-     dlrep l2 l2_head tail next nx) |-- !! (v0 = head) && emp *
-        dlrep (l1 ++ (v, p0) :: (z0, v1) :: l2) l1_head tail v0 nx *
-        data_at Tsh t_struct_node (Vint (Int.repr z), (pv, l1_head)) v0).
-        - entailer!.
-          pose proof elem_left_dlrep.
-          specialize (H0 l2 z0 next next tail p0 nx l2_head).
-          assert_PROP (data_at Tsh t_struct_node (Vint (Int.repr z0), (p0, l2_head)) next *
-     dlrep l2 l2_head tail next nx |-- !! (next = next) && emp * dlrep l2 l2_head tail next nx *
-         data_at Tsh t_struct_node (Vint (Int.repr z0), (p0, l2_head)) next).
-          entailer!. entailer!.
-          sep_apply H1; clear H1.
-          sep_apply H0; clear H0.
-          reflexivity.
-          entailer!.
-          specialize (IHl1 l1_head tail head nx prev next p0 v).
-          sep_apply IHl1; clear IHl1.
-          entailer!.
-        - sep_apply H2; clear H2. sep_apply H; clear H. exact H0.
-        entailer!.
-    Qed.
-        
-      
-    Lemma dlrep_middle_elem: forall l1 v p l2 head tail pv nx, 
-      
-          dlrep (l1 ++ (v,p) :: l2) head tail pv nx |-- EX prev next,
-            dlrep l1 head prev pv p * 
-            data_at Tsh t_struct_node (Vint (Int.repr v), (prev, next)) p *
-            dlrep l2 next tail p nx.
-       
-    Proof.
-      intros.
-      
-      revert head tail pv nx.
-      induction l1, l2; intros; autorewrite with sublist; unfold dlrep; fold dlrep.
-      + 
-        Intros next.
-        Exists pv nx.
-        entailer!.
-      +  
-       Intros next.
-        Exists pv next.
-        entailer!.
-      + 
-        assert ((a :: l1) ++ [(v,p)] = a :: (l1 ++ [(v,p)])).
-        list_solve.
-        rewrite H.
-        pose proof dlrep_left_elem.
-        destruct a.
-        specialize (H0 (l1++[(v,p)]) z v0 head tail pv nx).
+      * sep_apply H1.
         sep_apply H0.
-        clear  H0.
-        Intros next.
-        specialize (IHl1 next tail v0 nx).
+        { reflexivity. }
+
+        entailer!.
+        specialize (IHl1 l1_head tail head next prev' next' p0 x).
         sep_apply IHl1.
-        Intros prev next0.
-        Exists prev next0.
-        Exists next.
-        unfold dlrep; fold dlrep.
         entailer!.
-      + pose proof dlrep_left_elem.
-        destruct a.
-        assert (((z, v0) :: l1) ++ (v, p) :: p0 :: l2 = (z, v0) :: l1 ++ (v, p) :: p0 :: l2).
-        list_solve.
-        rewrite H0; clear H0.
-        specialize (H (l1 ++ (v, p) :: p0 :: l2) z v0 head tail pv nx).
-        sep_apply H.
-        Intros next.
-        specialize (IHl1 next tail v0 nx).
-        sep_apply IHl1.
-        Intros prev next0.
-        Exists prev next0.
-        Exists next.
-        destruct p0.
-        pose proof dlrep_left_elem.
-        specialize (H1 l2 z0 v1 next0 tail p nx).
-        sep_apply H1.
-        Intros next1.
-        Exists next1.
-        entailer!.
-    Qed.
-    
-    (* mallocN *)
-    Definition mallocN_spec :=
-     DECLARE _mallocN
-      WITH n: Z
-      PRE [tint]
-        PROP ( 4 <= n <= Int.max_unsigned )
-        PARAMS (Vint (Int.repr n))
-        GLOBALS ()
-        SEP ()
-      POST [ tptr tvoid ]
-        EX v: val,
-          PROP (malloc_compatible n v)
-          RETURN (v)
-          SEP (memory_block Tsh n v).
-    
-    (* freeN *)
-    Definition freeN_spec :=
-     DECLARE _freeN
-      WITH p : val , n : Z
-      PRE [ tptr tvoid , tint ]
-        PROP()
-        PARAMS (p; Vint (Int.repr n))
-        GLOBALS ()
-        SEP (memory_block Tsh n p)
-      POST [ tvoid ]
-        PROP () RETURN () SEP ().
-    
-    (* list_new *)
-    Definition list_new_spec :=
-     DECLARE _list_new
-      WITH u : unit
-      PRE  [  ]
-           PROP() PARAMS () GLOBALS () SEP ()
-      POST [ tptr t_struct_list ]
-        EX v: val,
-          PROP ()
-          RETURN (v)
-          SEP (list_rep nil v).
-          
-    Definition Gprog_list_new : funspecs := ltac:(with_library prog [list_new_spec; mallocN_spec]).
-    
-    Check memory_block_zero.
-    Check memory_block_isptr.
-    Check memory_block_split.
-    Check memory_block_data_at_.
-    
-    Lemma body_list_new: semax_body Vprog Gprog_list_new f_list_new list_new_spec.
-    Proof.
-      start_function.
-      
-      forward_call ((sizeof(Tstruct _list noattr))%expr).
-      {
-        simpl.
-        rep_lia.
-      }
-      Intros vert.
-      pose proof memory_block_data_at_ Tsh (Tstruct _list noattr) vert.
-      pose proof malloc_compatible_field_compatible. 
-      assert_PROP (complete_legal_cosu_type (Tstruct _list noattr) = true).
-      entailer!.
-      assert_PROP (natural_aligned natural_alignment (Tstruct _list noattr) = true).
-      entailer!.
-      specialize (H1 _ (Tstruct _list noattr) vert).
-      assert (field_compatible (Tstruct _list noattr) [] vert).
-      tauto.
-      assert (memory_block Tsh (sizeof (Tstruct _list noattr)) vert =
-         data_at_ Tsh (Tstruct _list noattr) vert).
-      tauto.
-      rewrite H5.
-      forward.
-      forward.
-      forward.
-      Exists vert.
-      entailer!.
-      unfold list_rep.
-      Exists (@nil (Z * val)).
-      entailer!.
-      unfold list_rep_with_cursor.
-      Exists nullval nullval.
-      unfold dlrep.
-      entailer!.
-    Qed.
-    (* list_free *)
-    Definition list_free_spec :=
-     DECLARE _list_free
-      WITH p : val, l : list Z
-      PRE  [ tptr t_struct_list ]
-        PROP () 
-        PARAMS (p) 
-        SEP (list_rep l p)
-      POST [ Tvoid ]
-        PROP ()
-        RETURN ()
-        SEP ().
-        
-    Definition Gprog_list_free : funspecs := ltac:(with_library prog [list_free_spec; freeN_spec]).
-    
-    
-    (* dlrep_ipon: for a list which represent a whole dlinklist,
-                   the corresponding head pointer will always be 
-                   `is_pointer_or_null` 
-                   
-       PS: ipon means: is pointer or null. *)
-    Lemma dlrep_ipon (l: list (Z * val)) (head tail : val):
-      dlrep l head tail nullval nullval |-- !! (is_pointer_or_null head ) && emp * dlrep l head tail nullval nullval.
-    Proof.
-      destruct l.
-      unfold dlrep.
-      
-      entailer!.
-      unfold dlrep. fold dlrep. destruct p. 
-      Intros head'.
-      Exists head'.
-      entailer!.
-    Qed.
-    
-    
-    (* dlrep_hdptr: the head pointer of l is head if pv=nx=nullval *)
-    Lemma dlrep_hdptr (l: list (Z * val)) (head tail: val):
-      dlrep l head tail nullval nullval |-- !!(head_ptr l = head) && emp * dlrep l head tail nullval nullval.
-    Proof.
-      destruct l.
-      unfold dlrep.
-      unfold head_ptr. unfold head_with_default. unfold map. entailer!.
-      unfold dlrep. fold dlrep. destruct p.
-      Intros head'. Exists head'.
-      unfold head_ptr.
-      unfold head_with_default. unfold map. unfold snd. entailer!.
-    Qed.
-    
-    
-    Lemma body_list_free: semax_body Vprog Gprog_list_new f_list_free list_free_spec.
-    Proof.
-      start_function.
-      unfold list_rep. unfold list_rep_with_cursor.
-      Intros l0 head tail.
-      forward.
-      sep_apply dlrep_ipon.
-      entailer!.
-      (* TODO: FIND THE LOOP INVARIANT *)
-    Abort.
-     
-    (* begin *)
-    Definition begin_spec :=
-     DECLARE _begin
-      WITH p : val, l : list (Z * val)
-      PRE  [ tptr t_struct_list ]
-        PROP () 
-        PARAMS (p)
-        GLOBALS ()
-        SEP (list_rep_with_cursor l p)
-      POST [ tptr t_struct_node ]
-        PROP ()
-        RETURN (head_ptr l)
-        SEP (list_rep_with_cursor l p).
-        
-    Definition Gprog_begin : funspecs := ltac:(with_library prog [begin_spec]).
-    
-    Lemma body_begin: semax_body Vprog Gprog_begin f_begin begin_spec.
-    Proof.
-      start_function.
-      unfold list_rep_with_cursor.
-      Intros head tail.
-      forward.
-      sep_apply dlrep_ipon.
-      entailer!.
-      forward.
-      unfold list_rep_with_cursor.
-      sep_apply dlrep_hdptr.
-      Exists head tail.
-      entailer!.
-    Qed.
-    
-    (* end *)
-    Definition end_spec :=
-     DECLARE _end
-      WITH p : val, l : list (Z * val)
-      PRE  [ tptr t_struct_list ]
-        PROP () 
-        PARAMS (p) 
-        GLOBALS ()
-        SEP (list_rep_with_cursor l p)
-      POST [ tptr t_struct_node ]
-        PROP ()
-        RETURN (nullval)
-        SEP (list_rep_with_cursor l p).
-        
-    Definition Gprog_end : funspecs := ltac:(with_library prog [end_spec]).
-    
-    Lemma body_end: semax_body Vprog Gprog_end f_end end_spec.
-    Proof.
-      start_function.
-      unfold list_rep_with_cursor.
-      Intros head tail.
-      forward.
-      unfold list_rep_with_cursor.
-      Exists head tail.
-      entailer!.
-    Qed.
-    
-    (* rbegin *)
-    Definition rbegin_spec :=
-     DECLARE _rbegin
-      WITH p : val, l : list (Z * val)
-      PRE  [ tptr t_struct_list ]
-        PROP () 
-        PARAMS (p) 
-        GLOBALS ()
-        SEP (list_rep_with_cursor l p)
-      POST [ tptr t_struct_node ]
-        PROP ()
-        RETURN (tail_ptr l)
-        SEP (list_rep_with_cursor l p).
-        
-    Definition Gprog_rbegin : funspecs := ltac:(with_library prog [rbegin_spec]).
-    
-    
-    (* llr: if a list l can be represent by a::l', 
-            then it can also be represent by l''++[b]. *)
-    Lemma llr  (l: list (Z*val)) (a: (Z*val)):
-      exists b l', a::l=l'++[b].
-    Proof.
-      pose proof classic (l=[]).
-      destruct H.
-      exists a,(@nil (Z*val)).
-      rewrite H.
-      list_solve.
-      exists (last l a), ([a]++(removelast l)).
-      pose proof app_removelast_last.
-      
-      assert (l = removelast l ++ [last l a]).
-      eapply H0.
-      exact H.
-      simpl.
-      rewrite <- H1.
-    
-      reflexivity.
-    Qed.
-    
-    (* the tail ptr of the list l is its tail *)
-    Lemma dlrep_tlptr (l: list (Z * val)) (head tail: val):
-      dlrep l head tail nullval nullval |-- !!(tail_ptr l = tail) && emp * dlrep l head tail nullval nullval.
-    Proof.
-      destruct l.
-      + unfold dlrep; fold dlrep.
-         unfold tail_ptr. unfold rev,map,snd,head_with_default.
-         entailer!.
-      + pose proof llr.
-        
-        destruct p.
-        
-        unfold tail_ptr.
-        unfold rev,map,snd,head_with_default.
-        unfold dlrep; fold dlrep.
-        Intros head'.
-        Exists head'.
-        entailer!.
-        (*TODO: tail_ptr: fuck u. *)
-    Abort.
-    
-    (* similar with dlrep_ipon, but this time is: is_pointer_or_null tail *)
-    Lemma dlrep_ipon2 (l: list (Z * val)) (head tail : val):
-      dlrep l head tail nullval nullval |-- !! (is_pointer_or_null tail ) && emp * dlrep l head tail nullval nullval.
-    Proof.
-      destruct l.
-      unfold dlrep.
-      
-      entailer!.
-      pose proof llr.
-      specialize (H l p).
-      destruct H as [y [l']].
-      rewrite H.
-      pose proof dlrep_right_elem.
-      destruct y.
-      sep_apply dlrep_right_elem.
-      Intros prev.
-      entailer!.
-      pose proof elem_right_dlrep.
-      specialize (H1 l' z tail head tail nullval nullval prev).
-      assert_PROP (
-        dlrep l' head prev nullval tail *
-    data_at Tsh t_struct_node (Vint (Int.repr z), (prev, nullval)) tail |--
-        !! (tail = tail) && emp * dlrep l' head prev nullval tail *
-         data_at Tsh t_struct_node (Vint (Int.repr z), (prev, nullval)) tail
-      ).
-      entailer!.
-      sep_apply H4.
-      sep_apply H1.
-      reflexivity.
-      entailer!.
-    Qed.
-    
-    Lemma body_rbegin: semax_body Vprog Gprog_end f_rbegin rbegin_spec.
-    Proof.
-      start_function.
-      unfold list_rep_with_cursor.
-      Intros head tail.
-      forward.
-      sep_apply dlrep_ipon2.
-      entailer!.
-      forward.
-      (*TODO: fix the holes of the previous lemma, then this will be solved. *)
-    Abort.
-    
-    (* rend *)
-    Definition rend_spec :=
-     DECLARE _rend
-      WITH p : val, l : list (Z * val)
-      PRE  [ tptr t_struct_list ]
-        PROP () 
-        PARAMS (p) 
-        GLOBALS ()
-        SEP (list_rep_with_cursor l p)
-      POST [ tptr t_struct_node ]
-        PROP ()
-        RETURN (nullval)
-        SEP (list_rep_with_cursor l p).
-    
-    (* next *)
-    Definition next_spec :=
-     DECLARE _next
-      WITH l1 : list (Z * val), v: Z, p: val, l2 : list (Z * val), x: val
-      PRE  [ tptr t_struct_node ]
-        PROP () 
-        PARAMS (p)
-        GLOBALS ()
-        SEP (list_rep_with_cursor (l1 ++ [(v, p)] ++ l2) x)
-      POST [ tptr t_struct_node ]
-        PROP ()
-        RETURN (head_ptr l2)
-        SEP (list_rep_with_cursor (l1 ++ [(v, p)] ++ l2) x).
-    
-    (* rnext *)
-    Definition rnext_spec :=
-     DECLARE _rnext
-      WITH l1 : list (Z * val), v: Z, p: val, l2 : list (Z * val), x: val
-      PRE  [ tptr t_struct_node ]
-        PROP () 
-        PARAMS (p)
-        GLOBALS ()
-        SEP (list_rep_with_cursor (l1 ++ [(v, p)] ++ l2) x)
-      POST [ tptr t_struct_node ]
-        PROP ()
-        RETURN (tail_ptr l1)
-        SEP (list_rep_with_cursor (l1 ++ [(v, p)] ++ l2) x).
-    
-    (* get_val *)
-    Definition get_val_spec :=
-     DECLARE _get_val
-      WITH l1 : list (Z * val), v: Z, p: val, l2 : list (Z * val), x: val
-      PRE  [ tptr t_struct_node ]
-        PROP () 
-        PARAMS (p)
-        GLOBALS ()
-        SEP (list_rep_with_cursor (l1 ++ [(v, p)] ++ l2) x)
-      POST [ tuint ]
-        PROP ()
-        RETURN (Vint (Int.repr v))
-        SEP (list_rep_with_cursor (l1 ++ [(v, p)] ++ l2) x).
-        
-    Definition Gprog_get_val : funspecs := ltac:(with_library prog [get_val_spec]).
-    
-    (* dlrep (l1 ++ (v, p) :: l2) head tail
-         nullval nullval))
-       ==> convert to: dlrep l1 head tail' nullval nullval * data_at (v, p) * dlrep l2 head' tail nullval nullval *)
-    
-        
-    
-    Lemma body_get_val: semax_body Vprog Gprog_get_val f_get_val get_val_spec.
-    Proof.
-      start_function.
-      unfold MORE_COMMANDS, abbreviate.
-      unfold list_rep_with_cursor.
-      Intros head tail.
-      unfold dlrep. fold dlrep.
-      pose proof dlrep_middle_elem.
-      specialize (H l1 v p l2 head tail nullval nullval).
+    - sep_apply H2.
       sep_apply H.
-      Intros prev next.
-      forward.
-      forward.
-      unfold list_rep_with_cursor.
-      Exists head tail.
-      sep_apply elem_middle_dlrep.
-      
-      
+      { exact H0. }
       entailer!.
-    Qed.
-    
-    (* 2021-04-27 01:16 *)
-    
+Qed.
+
+Lemma dlrep_local_facts_head:
+  forall l head tail,
+    dlrep l head tail nullval nullval |--
+    !! (is_pointer_or_null head) && emp * dlrep l head tail nullval nullval.
+Proof.
+  intros.
+  destruct l.
+  + unfold dlrep.
+    entailer!.
+  + unfold dlrep; fold dlrep.
+    destruct p. 
+    Intros head'.
+    Exists head'.
+    entailer!.
+Qed.
+
+Lemma dlrep_local_facts_tail:
+  forall l head tail,
+    dlrep l head tail nullval nullval |--
+    !! (is_pointer_or_null tail ) && emp * dlrep l head tail nullval nullval.
+Proof.
+  destruct l.
+  unfold dlrep.
+  { entailer!. }
+  
+Admitted.
+
+(** Memory representation of a mathematical list. Cursors mean places to
+    insert. *)
+Definition list_rep_with_cursor (l : list (Z * val)) (p : val) : mpred :=
+  EX (head tail : val),
+    data_at Tsh t_struct_list (head, tail) p *
+      dlrep l head tail nullval nullval.
+
+Definition list_rep (l : list Z) (p : val) : mpred :=
+  EX l0: list (Z * val),
+    !! (map fst l0 = l) && list_rep_with_cursor l0 p.
+
+(** Head pointer and tail pointer *)
+Definition head_with_default {A: Type} (l: list A) (default: A): A :=
+  match l with
+  | a :: _ => a
+  | nil => default
+  end.
+
+Definition head_ptr (l : list (Z * val)): val :=
+  head_with_default (map snd l) nullval.
+  
+Definition tail_ptr (l : list (Z * val)): val :=
+  head_with_default (rev (map snd l)) nullval.
+
+Lemma dlrep_head_ptr:
+  forall l head tail,
+    dlrep l head tail nullval nullval |--
+    !!(head_ptr l = head) && emp * dlrep l head tail nullval nullval.
+Proof.
+  intros.
+  destruct l.
+  unfold dlrep.
+  unfold head_ptr, head_with_default, map.
+  entailer!.
+  unfold dlrep; fold dlrep.
+  destruct p.
+  Intros head'.
+  Exists head'.
+  unfold head_ptr.
+  unfold head_with_default, map, snd.
+  entailer!.
+Qed.
+
+Lemma dlrep_tail_ptr:
+  forall l head tail,
+    dlrep l head tail nullval nullval |--
+    !!(tail_ptr l = tail) && emp * dlrep l head tail nullval nullval.
+Proof.
+  intros.
+  destruct l.
+  + unfold dlrep; fold dlrep.
+    unfold tail_ptr, head_with_default, rev, map, snd.
+    entailer!.
+  + 
+
+Admitted.
+
+(** Specifications about memory operations *)
+
+(* mallocN *)
+Definition mallocN_spec :=
+ DECLARE _mallocN
+  WITH n: Z
+  PRE [tint]
+    PROP (4 <= n <= Int.max_unsigned)
+    PARAMS (Vint (Int.repr n))
+    GLOBALS ()
+    SEP ()
+  POST [ tptr tvoid ]
+    EX v: val,
+      PROP (malloc_compatible n v)
+      RETURN (v)
+      SEP (memory_block Tsh n v).
+
+(* freeN *)
+Definition freeN_spec :=
+ DECLARE _freeN
+  WITH p : val , n : Z
+  PRE [ tptr tvoid , tint ]
+    PROP()
+    PARAMS (p; Vint (Int.repr n))
+    GLOBALS ()
+    SEP (memory_block Tsh n p)
+  POST [ tvoid ]
+    PROP () RETURN () SEP ().
+
+(** Functions to be verified. *)
+
+(* list_new *)
+Definition list_new_spec :=
+ DECLARE _list_new
+  WITH u : unit
+  PRE  [  ]
+       PROP() PARAMS () GLOBALS () SEP ()
+  POST [ tptr t_struct_list ]
+    EX v: val,
+      PROP ()
+      RETURN (v)
+      SEP (list_rep nil v).
+
+Definition Gprog_list_new : funspecs :=
+            ltac:(with_library prog [list_new_spec; mallocN_spec]).
+
+Check memory_block_zero.
+Check memory_block_isptr.
+Check memory_block_split.
+Check memory_block_data_at_.
+
+Theorem body_list_new: semax_body Vprog Gprog_list_new
+                         f_list_new list_new_spec.
+Proof.
+  start_function.
+  
+  forward_call ((sizeof (Tstruct _list noattr))%expr).
+  {
+    simpl.
+    rep_lia.
+  }
+
+  Intros vert.
+  pose proof memory_block_data_at_ Tsh (Tstruct _list noattr) vert.
+  pose proof malloc_compatible_field_compatible. 
+  assert_PROP (complete_legal_cosu_type (Tstruct _list noattr) = true).
+  { entailer!. }
+
+  assert_PROP (natural_aligned natural_alignment (Tstruct _list noattr) = true).
+  { entailer!. }
+
+  specialize (H1 _ (Tstruct _list noattr) vert).
+  assert (field_compatible (Tstruct _list noattr) [] vert).
+  { tauto. }
+
+  assert (memory_block Tsh (sizeof (Tstruct _list noattr)) vert =
+      data_at_ Tsh (Tstruct _list noattr) vert).
+  { tauto. }
+
+  rewrite H5.
+  forward.
+  forward.
+  forward.
+  Exists vert.
+  entailer!.
+
+  unfold list_rep.
+  Exists (@nil (Z * val)).
+  entailer!.
+  unfold list_rep_with_cursor.
+  Exists nullval nullval.
+  unfold dlrep.
+  entailer!.
+Qed.
+
+(* list_free *)
+Definition list_free_spec :=
+ DECLARE _list_free
+  WITH p : val, l : list Z
+  PRE  [ tptr t_struct_list ]
+    PROP () 
+    PARAMS (p) 
+    SEP (list_rep l p)
+  POST [ Tvoid ]
+    PROP ()
+    RETURN ()
+    SEP ().
+
+Definition Gprog_list_free : funspecs :=
+            ltac:(with_library prog [list_free_spec; freeN_spec]).
+
+Theorem body_list_free: semax_body Vprog Gprog_list_new
+                          f_list_free list_free_spec.
+Proof.
+  start_function.
+
+  unfold list_rep, list_rep_with_cursor.
+  Intros l0 head tail.
+  forward.
+  sep_apply dlrep_local_facts_head.
+  entailer!.
+  (* TODO: Find the loop invariant. *)
+Admitted.
+
+(* begin *)
+Definition begin_spec :=
+ DECLARE _begin
+  WITH p : val, l : list (Z * val)
+  PRE  [ tptr t_struct_list ]
+    PROP () 
+    PARAMS (p)
+    GLOBALS ()
+    SEP (list_rep_with_cursor l p)
+  POST [ tptr t_struct_node ]
+    PROP ()
+    RETURN (head_ptr l)
+    SEP (list_rep_with_cursor l p).
+
+Definition Gprog_begin : funspecs :=
+            ltac:(with_library prog [begin_spec]).
+
+Theorem body_begin: semax_body Vprog Gprog_begin
+                      f_begin begin_spec.
+Proof.
+  start_function.
+  unfold list_rep_with_cursor.
+  Intros head tail.
+  forward.
+  sep_apply dlrep_local_facts_head.
+  entailer!.
+  forward.
+  unfold list_rep_with_cursor.
+  sep_apply dlrep_head_ptr.
+  Exists head tail.
+  entailer!.
+Qed.
+
+(* end *)
+Definition end_spec :=
+ DECLARE _end
+  WITH p : val, l : list (Z * val)
+  PRE  [ tptr t_struct_list ]
+    PROP () 
+    PARAMS (p) 
+    GLOBALS ()
+    SEP (list_rep_with_cursor l p)
+  POST [ tptr t_struct_node ]
+    PROP ()
+    RETURN (nullval)
+    SEP (list_rep_with_cursor l p).
+
+Definition Gprog_end : funspecs :=
+            ltac:(with_library prog [end_spec]).
+
+Theorem body_end: semax_body Vprog Gprog_end
+                    f_end end_spec.
+Proof.
+  start_function.
+  unfold list_rep_with_cursor.
+  Intros head tail.
+  forward.
+  unfold list_rep_with_cursor.
+  Exists head tail.
+  entailer!.
+Qed.
+
+(* rbegin *)
+Definition rbegin_spec :=
+ DECLARE _rbegin
+  WITH p : val, l : list (Z * val)
+  PRE  [ tptr t_struct_list ]
+    PROP () 
+    PARAMS (p) 
+    GLOBALS ()
+    SEP (list_rep_with_cursor l p)
+  POST [ tptr t_struct_node ]
+    PROP ()
+    RETURN (tail_ptr l)
+    SEP (list_rep_with_cursor l p).
+
+Definition Gprog_rbegin : funspecs :=
+            ltac:(with_library prog [rbegin_spec]).
+
+Theorem body_rbegin: semax_body Vprog Gprog_rbegin
+                       f_rbegin rbegin_spec.
+Proof.
+  start_function.
+  unfold list_rep_with_cursor.
+  Intros head tail.
+  forward.
+  sep_apply dlrep_local_facts_tail.
+  entailer!.
+  forward.
+  (* TODO: fix the holes of the previous lemma. *)
+Admitted.
+
+(* rend *)
+Definition rend_spec :=
+ DECLARE _rend
+  WITH p : val, l : list (Z * val)
+  PRE  [ tptr t_struct_list ]
+    PROP () 
+    PARAMS (p) 
+    GLOBALS ()
+    SEP (list_rep_with_cursor l p)
+  POST [ tptr t_struct_node ]
+    PROP ()
+    RETURN (nullval)
+    SEP (list_rep_with_cursor l p).
+
+Definition Gprog_rend : funspecs :=
+            ltac:(with_library prog [rend_spec]).
+
+Theorem body_rend: semax_body Vprog Gprog_rend
+                     f_rend rend_spec.
+Proof.
+
+Admitted.
+
+(* next *)
+Definition next_spec :=
+ DECLARE _next
+  WITH l1 : list (Z * val), v: Z, p: val, l2 : list (Z * val), x: val
+  PRE  [ tptr t_struct_node ]
+    PROP () 
+    PARAMS (p)
+    GLOBALS ()
+    SEP (list_rep_with_cursor (l1 ++ [(v, p)] ++ l2) x)
+  POST [ tptr t_struct_node ]
+    PROP ()
+    RETURN (head_ptr l2)
+    SEP (list_rep_with_cursor (l1 ++ [(v, p)] ++ l2) x).
+
+Definition Gprog_next : funspecs :=
+            ltac:(with_library prog [next_spec]).
+
+Theorem body_next: semax_body Vprog Gprog_next
+                     f_next next_spec.
+Proof.
+
+Admitted.
+
+(* rnext *)
+Definition rnext_spec :=
+ DECLARE _rnext
+  WITH l1 : list (Z * val), v: Z, p: val, l2 : list (Z * val), x: val
+  PRE  [ tptr t_struct_node ]
+    PROP () 
+    PARAMS (p)
+    GLOBALS ()
+    SEP (list_rep_with_cursor (l1 ++ [(v, p)] ++ l2) x)
+  POST [ tptr t_struct_node ]
+    PROP ()
+    RETURN (tail_ptr l1)
+    SEP (list_rep_with_cursor (l1 ++ [(v, p)] ++ l2) x).
+
+Definition Gprog_rnext : funspecs :=
+            ltac:(with_library prog [rnext_spec]).
+
+Theorem body_rnext: semax_body Vprog Gprog_rnext
+               f_rnext rnext_spec.
+Proof.
+
+Admitted.
+
+(* get_val *)
+Definition get_val_spec :=
+ DECLARE _get_val
+  WITH l1 : list (Z * val), v: Z, p: val, l2 : list (Z * val), x: val
+  PRE  [ tptr t_struct_node ]
+    PROP () 
+    PARAMS (p)
+    GLOBALS ()
+    SEP (list_rep_with_cursor (l1 ++ [(v, p)] ++ l2) x)
+  POST [ tuint ]
+    PROP ()
+    RETURN (Vint (Int.repr v))
+    SEP (list_rep_with_cursor (l1 ++ [(v, p)] ++ l2) x).
+
+Definition Gprog_get_val : funspecs :=
+            ltac:(with_library prog [get_val_spec]).
+
+Theorem body_get_val: semax_body Vprog Gprog_get_val
+                        f_get_val get_val_spec.
+Proof.
+  start_function.
+  unfold MORE_COMMANDS, abbreviate.
+  unfold list_rep_with_cursor.
+  Intros head tail.
+  unfold dlrep. fold dlrep.
+  pose proof dlrep_middle_elem.
+  specialize (H l1 v p l2 head tail nullval nullval).
+  sep_apply H.
+  Intros prev next.
+  forward.
+  forward.
+  unfold list_rep_with_cursor.
+  Exists head tail.
+  sep_apply elem_middle_dlrep.
+  entailer!.
+Qed.
+
+(* insert_before *)
+
+(* insert_after *)
+
+(* merge *)
+
+(** Functions to be verified. *)
+
+(* sum *)
+
+(* delta *)
+
+(* 2021-04-27 01:16 *)
